Stash

BW.hs
@@ -1,0 +1,29 @@
+import Data.List (sortOn, sort)
+
+lrot :: [a] -> [a]
+lrot [] = []
+lrot xs = tail xs ++ [head xs]
+
+rrot :: [a] -> [a]
+rrot [] = []
+rrot xs = last xs : init xs
+
+rots :: [a] -> [[a]]
+rots xs = take (length xs) $ iterate lrot xs
+
+printMat :: [String] -> IO ()
+printMat = mapM_ putStrLn
+
+sortFrom :: Int -> [String] -> [String]
+sortFrom 0 m = sortOn (!! i') $ m
+    where i' = length m - 1
+sortFrom i m = sortOn (!! i') $ sortFrom (i-1) m
+    where i' = length m - 1 - i
+
+bwp :: Ord a => [a] -> [a]
+bwp = map last . sort . rots
+
+recreate :: Ord a => Int -> [a] -> [[a]]
+recreate 0 l = map (const []) l
+recreate j l = sortOn head . zipWith (:) l $ recreate (j-1) l
+
